specs/Spec.Agile.Cipher.fst
@@ -7,20 +7,26 @@ open Lib.ByteSequence
 
 #reset-options "--z3rlimit 20 --max_fuel 0 --max_ifuel 1"
 
-/// This module is concerned with defining an agile stream cipher, i.e. a
-/// function that given: a suitably extended key; an iv (nonce); a counter,
-/// produces a fresh block.
-///
-/// TODO: share definitions with Spec.AEAD, in particular definitions of nonce,
-/// key, key expansion, etc.
-
 let aes_ctr_block_add_counter (block: lbytes 16) (incr:size_nat): Tot (lbytes 16) =
   let n = nat_from_bytes_be block in
   let n' = (n + incr) % pow2 128 in
   nat_to_bytes_be 16 n'
 
+let xkey (a: cipher_alg) =
+  match a with
+  | AES128 | AES256 -> Spec.AES.aes_xkey (aes_alg_of_alg a)
+  | CHACHA20 -> Spec.Chacha20.key
+
+/// As specified by the NIST. Other implementations (e.g. Vale) may perform
+/// other steps beyond key expansion but this is an implementation detail.
+let expand (a: cipher_alg) (k: key a): xkey a =
+  match a with
+  | AES128 | AES256 -> Spec.AES.aes_key_expansion (aes_alg_of_alg a) k
+  | CHACHA20 -> k
+
 /// A block is a function of key, iv, counter.
-let ctr_block (a: cipher_alg) (k: xkey a) (iv: nonce a) (c: ctr): block a =
+let ctr_block (a: cipher_alg) (k: key a) (iv: nonce a) (c: ctr): block a =
+  let k = expand a k in
   match a with
   | AES128 | AES256 ->
       let open Spec.AES in
