specs/Spec.Agile.Cipher.fsti
@@ -8,11 +8,12 @@ open Lib.ByteSequence
 #reset-options "--z3rlimit 20 --max_fuel 0 --max_ifuel 1"
 
 /// This module is concerned with defining an agile stream cipher, i.e. a
-/// function that given: a suitably extended key; an iv (nonce); a counter,
-/// produces a fresh block.
-///
-/// TODO: share definitions with Spec.AEAD, in particular definitions of nonce,
-/// key, key expansion, etc.
+/// function that given: a key; an iv (nonce); a counter, produces a fresh
+/// block. We leave details of key expansion to the ``.fst``, or possibly even
+/// to the low-level implementation.
+
+/// Definitions
+/// -----------
 
 type cipher_alg =
   | AES128
@@ -26,24 +27,26 @@ let aes_alg_of_alg (a: cipher_alg { a = AES128 \/ a = AES256 }) =
   | AES128 -> Spec.AES.AES128
   | AES256 -> Spec.AES.AES256
 
-/// Algorithms may (AES) or may not (Chacha) require a preliminary round of key expansion.
-let xkey (a: cipher_alg) =
-  match a with
-  | AES128 | AES256 -> Spec.AES.aes_xkey (aes_alg_of_alg a)
-  | CHACHA20 -> Spec.Chacha20.key
-
 /// Trying to enforce conventions: lengths for nats (spec); len for machine
 /// integers (runtime).
+let key_length (a: cipher_alg): size_nat =
+  match a with
+  | AES128 | AES256 -> Spec.AES.key_size (aes_alg_of_alg a)
+  | CHACHA20 -> Spec.Chacha20.size_key
+
+let key (a: cipher_alg) =
+  match a with
+  | AES128 | AES256 -> Spec.AES.aes_key (aes_alg_of_alg a)
+  | CHACHA20 -> Spec.Chacha20.key
+
 let block_length (a:cipher_alg) =
   match a with
   | AES128 | AES256 -> 16
   | CHACHA20 -> 64
 
-/// Type abbreviations.
 let block a = lbytes (block_length a)
 
-let ctr = size_nat
-
+/// Smaller bound than for AES-GCM; no IV reduction.
 let nonce_bound (a: cipher_alg) (n_len: nat): Type0 =
   match a with
   | AES128 | AES256 -> n_len <= block_length a
@@ -51,11 +54,18 @@ let nonce_bound (a: cipher_alg) (n_len: nat): Type0 =
 
 let nonce a = b:bytes { nonce_bound a (length b) }
 
-val ctr_block (a: cipher_alg) (k: xkey a) (iv: nonce a) (c: ctr): block a
+let ctr = size_nat
+
+
+/// The stream cipher
+/// -----------------
+
+/// One block of pseudo-random bytes.
+val ctr_block (a: cipher_alg) (k: key a) (iv: nonce a) (c: ctr): block a
 
 /// A stream of pseudo-random bytes, starting from counter zero. The length is
 /// artificially constrained to be < 2^32.
-let ctr_stream (a: cipher_alg) (k: xkey a) (iv: nonce a) (len: size_nat):
+let ctr_stream (a: cipher_alg) (k: key a) (iv: nonce a) (len: size_nat):
   b:bytes { length b = len }
 =
   // JP: useful? be overconservative and always do + 1? would necessitate a
@@ -77,6 +87,10 @@ let ctr_stream (a: cipher_alg) (k: xkey a) (iv: nonce a) (len: size_nat):
   in
   Seq.slice blocks 0 len
 
+
+/// TODO
+/// ----
+///
 /// Possible addition: ctr_stream_n, which generates ``len`` bytes starting from
 /// counter ``n`` (or, possibly, from bytes ``n``). I don't think it's necessary
 /// to have that one to properly specify ``EverCrypt.CTR``.
