providers/evercrypt/fst/EverCrypt.CTR.fst
@@ -1,0 +1,76 @@
+module EverCrypt.CTR
+
+module ST = FStar.HyperStack.ST
+module HS = FStar.HyperStack
+module B = LowStar.Buffer
+module G = FStar.Ghost
+
+module Spec = Spec.Agile.CTR
+
+open FStar.HyperStack.ST
+open LowStar.BufferOps
+
+let uint8 = Lib.IntTypes.uint8
+let uint32 = Lib.IntTypes.uint32
+let buffer8 = B.buffer uint8
+
+/// Some implementations may choose to reserve more space in the expanded key
+/// for other pre-computations.
+let concrete_xkey_length: cipher_alg -> size_nat =
+  function
+  | CHACHA20 -> 32
+  | AES128 -> 176 + 128 // Include the hashed keys here
+  | AES256 -> 240 + 128 // Include the hashed keys here
+
+
+let expand (#a: supported_alg) (k: kv a): ekv a =
+  match a with
+  | CHACHA20_POLY1305 -> k
+  | AES256_GCM | AES128_GCM ->
+      let open Vale.AES.AES_s in
+      assert_norm (32 % 4 = 0);
+      assert_norm (16 % 4 = 0);
+      let k_nat = Vale.Def.Words.Seq_s.seq_uint8_to_seq_nat8 k in
+      let k_w = Vale.Def.Words.Seq_s.seq_nat8_to_seq_nat32_LE k_nat in
+      let ekv_w = key_to_round_keys_LE (vale_alg_of_alg a) k_w in
+      let ekv_nat = Vale.Def.Types_s.le_seq_quad32_to_bytes ekv_w in
+      Vale.Def.Types_s.le_seq_quad32_to_bytes_length ekv_w;
+      let ek = Vale.Def.Words.Seq_s.seq_nat8_to_seq_uint8 ekv_nat in
+      let hkeys_quad = Vale.AES.OptPublic.get_hkeys_reqs (Vale.Def.Types_s.reverse_bytes_quad32 (
+        aes_encrypt_LE (vale_alg_of_alg a) k_w (Vale.Def.Words_s.Mkfour 0 0 0 0))) in
+      let hkeys = Vale.Def.Words.Seq_s.seq_nat8_to_seq_uint8 (Vale.Def.Types_s.le_seq_quad32_to_bytes hkeys_quad) in
+      Seq.append ek hkeys
+
+
+
+/// Duplicated with EverCrypt.AEAD. Unify?
+type impl =
+  | Vale_AES128
+  | Vale_AES256
+  | Hacl_CHACHA20
+
+noeq
+type state_s (a: Spec.cipher_alg) =
+| State:
+    impl:impl ->
+    g_iv: G.erased (Spec.nonce a) ->
+    iv: buffer8 { Spec.nonce_bound a (B.length iv) } ->
+    g_key: G.erased (Spec.xkey a) ->
+    xkey: buffer8 { B.length xkey = Spec.concrete_xkey_length a } ->
+    ctr: uint32 ->
+    state_s a
+
+let freeable_s #a s =
+  let State _ _ iv _ key _ = s in
+  B.freeable iv /\ B.freeable key
+
+let footprint_s #a s =
+  let State _ _ iv _ key _ = s in
+  B.(loc_addr_of_buffer iv `loc_union` loc_addr_of_buffer key)
+
+let invariant_s #a h s =
+  let State impl g_iv iv g_key key _ = s in
+  B.live h iv /\ B.live h key /\
+  G.reveal g_iv `Seq.equal` B.as_seq h iv /\
+  G.reveal g_key `Seq.equal` B.as_seq h key /\
+  true
