specs/Spec.AES.Vale.fsti
@@ -1,0 +1,14 @@
+module Spec.AES.Vale
+
+open Spec.Agile.Cipher
+
+let vale_cipher_alg = a: cipher_alg { a == AES128 \/ a == AES256 }
+
+/// Vale-specific AES key expansion precomputed with powers of H. Shared between
+/// CTR and GCM, hence in a separate module.
+val vale_aes_expansion (a: vale_cipher_alg) (key: key a):
+  Lib.ByteSequence.bytes
+
+/// Vale-specific extended key length in the concrete representation with space
+/// for other precomputer things.
+val vale_xkey_length (a: vale_cipher_alg): nat
